messing around with interp and its soundness wrt small-step

theories/effects/delim.v
@@ -27,7 +27,25 @@ Program Definition resetE : opInterp :=
   |}.
 
 (* to apply the head of the meta continuation *)
-Program Definition popE : opInterp :=
+Program Definition pop_apply_E : opInterp :=
+  {|
+    Ins := (▶ ∙);
+    Outs := Empty_setO;
+  |}.
+
+Program Definition peek_apply_E : opInterp :=
+  {|
+    Ins := (▶ ∙);
+    Outs := Empty_setO;
+  |}.
+
+Program Definition pop_continue_E : opInterp :=
+  {|
+    Ins := (▶ ∙);
+    Outs := (▶ ∙);
+  |}.
+
+Program Definition pop_discard_E : opInterp :=
   {|
     Ins := (▶ ∙);
     Outs := Empty_setO;
@@ -40,12 +58,29 @@ Program Definition appContE : opInterp :=
     Outs := ▶ ∙;
   |} .
 
-Definition delimE := @[shiftE; resetE; popE;appContE].
+Program Definition shiftE' : opInterp :=
+  {|
+    Ins := ((▶ ∙ -n> ▶ ∙) -n> ▶ ∙);
+    Outs := (▶ ∙);
+  |}.
 
-Notation op_shift := (inl ()).
-Notation op_reset := (inr (inl ())).
-Notation op_pop := (inr (inr (inl ()))).
-Notation op_app_cont := (inr (inr (inr (inl ())))).
+Definition delimE := @[shiftE
+                       ; resetE
+                       ; pop_apply_E
+                       ; peek_apply_E
+                       ; pop_continue_E
+                       ; pop_discard_E
+                       ; appContE
+                       ; shiftE'].
+
+Notation op_shift        := (inl ()).
+Notation op_reset        := (inr (inl ())).
+Notation op_pop_apply    := (inr (inr (inl ()))).
+Notation op_peek_apply   := (inr (inr (inr (inl ())))).
+Notation op_pop_continue := (inr (inr (inr (inr (inl ()))))).
+Notation op_pop_discard  := (inr (inr (inr (inr (inr (inl ())))))).
+Notation op_app_cont     := (inr (inr (inr (inr (inr (inr (inl ()))))))).
+Notation op_shift'       := (inr (inr (inr (inr (inr (inr (inr (inl ())))))))).
 
 Section reifiers.
   Context {X} `{!Cofe X}.
@@ -71,20 +106,57 @@ Section reifiers.
         optionO (prodO (laterO X) state)).
   Proof. intros ?[[]][[]][[]]. simpl in *. by repeat f_equiv. Qed.
 
-
-  Definition reify_pop : (laterO X) * state * (Empty_setO -n> laterO X) →
-                           option (laterO X * state) :=
+  Definition reify_pop_apply : (laterO X) * state * (Empty_setO -n> laterO X) →
+                               option (laterO X * state) :=
     λ '(e, σ, _),
       match σ with
       | [] => Some (e, σ)
       | k' :: σ' => Some (k' e, σ')
       end.
-  #[export] Instance reify_pop_ne :
-    NonExpansive (reify_pop :
+  #[export] Instance reify_pop_apply_ne :
+    NonExpansive (reify_pop_apply :
         prodO (prodO (laterO X) state) (Empty_setO -n> laterO X) →
         optionO (prodO (laterO X) state)).
   Proof. intros ?[[]][[]][[]]. simpl in *. by repeat f_equiv. Qed.
 
+  Definition reify_peek_apply : (laterO X) * state * (Empty_setO -n> laterO X) →
+                           option (laterO X * state) :=
+    λ '(e, σ, _),
+      match σ with
+      | [] => Some (e, σ)
+      | k' :: σ' => Some (k' e, k' :: σ')
+      end.
+  #[export] Instance reify_peek_apply_ne :
+    NonExpansive (reify_peek_apply :
+        prodO (prodO (laterO X) state) (Empty_setO -n> laterO X) →
+        optionO (prodO (laterO X) state)).
+  Proof. intros ?[[]][[]][[]]. simpl in *. by repeat f_equiv. Qed.
+
+  Definition reify_pop_continue : (laterO X) * state * (laterO X -n> laterO X) →
+                                  option (laterO X * state) :=
+    λ '(e, σ, κ),
+      match σ with
+      | [] => Some (κ e, σ)
+      | _ :: σ' => Some (κ e, σ')
+      end.
+  #[export] Instance reify_pop_continue_ne :
+    NonExpansive (reify_pop_continue :
+        prodO (prodO (laterO X) state) (laterO X -n> laterO X) →
+        optionO (prodO (laterO X) state)).
+  Proof. intros ?[[]][[]][[]]. simpl in *. by repeat f_equiv. Qed.
+
+  Definition reify_pop_discard : (laterO X) * state * (Empty_setO -n> laterO X) →
+                                 option (laterO X * state) :=
+    λ '(e, σ, _),
+      match σ with
+      | [] => Some (e, σ)
+      | _ :: σ' => Some (e, σ')
+      end.
+  #[export] Instance reify_pop_discard_ne :
+    NonExpansive (reify_pop_discard :
+        prodO (prodO (laterO X) state) (Empty_setO -n> laterO X) →
+        optionO (prodO (laterO X) state)).
+  Proof. intros ?[[]][[]][[]]. simpl in *. by repeat f_equiv. Qed.
 
   Definition reify_app_cont : ((laterO X * (laterO (X -n> X))) * state * (laterO X -n> laterO X)) →
                               option (laterO X * state) :=
@@ -100,6 +172,17 @@ Section reifiers.
     repeat f_equiv; apply H.
   Qed.
 
+  Definition reify_shift' : ((laterO X -n> laterO X) -n> laterO X) *
+                              state * (laterO X -n> laterO X) →
+                            option (laterO X * state) :=
+    λ '(f, σ, k), Some ((f k): laterO X, tail (σ : state)).
+  #[export] Instance reify_shift_ne' :
+    NonExpansive (reify_shift' :
+      prodO (prodO ((laterO X -n> laterO X) -n> laterO X) state)
+        (laterO X -n> laterO X) →
+      optionO (prodO (laterO X) state)).
+  Proof. intros ?[[]][[]][[]]. simpl in *. repeat f_equiv; auto. Qed.
+
 End reifiers.
 
 Canonical Structure reify_delim : sReifier CtxDep.
@@ -109,11 +192,15 @@ Proof.
              sReifier_state := stateF
            |}.
   intros X HX op.
-  destruct op as [ | [ | [ | [| []]]]]; simpl.
+  destruct op as [ | [ | [ | [| [| [| [| [| []]]]]]]]]; simpl.
   - simple refine (OfeMor (reify_shift)).
   - simple refine (OfeMor (reify_reset)).
-  - simple refine (OfeMor (reify_pop)).
+  - simple refine (OfeMor (reify_pop_apply)).
+  - simple refine (OfeMor (reify_peek_apply)).
+  - simple refine (OfeMor (reify_pop_continue)).
+  - simple refine (OfeMor (reify_pop_discard)).
   - simple refine (OfeMor (reify_app_cont)).
+  - simple refine (OfeMor (reify_shift')).
 Defined.
 
 Section constructors.
@@ -126,13 +213,37 @@ Section constructors.
 
   (** ** POP *)
 
-  Program Definition POP : IT -n> IT :=
-    λne e, Vis (E:=E) (subEff_opid op_pop)
-             (subEff_ins (F:=delimE) (op:=op_pop) (Next e))
-             (Empty_setO_rec _ ◎ (subEff_outs (F:=delimE) (op:=op_pop))^-1).
+  Program Definition POP_APPLY : IT -n> IT :=
+    λne e, Vis (E:=E) (subEff_opid op_pop_apply)
+             (subEff_ins (F:=delimE) (op:=op_pop_apply) (Next e))
+             (Empty_setO_rec _ ◎ (subEff_outs (F:=delimE) (op:=op_pop_apply))^-1).
   Solve All Obligations with solve_proper.
 
-  Notation 𝒫 := (get_val POP).
+  Program Definition PEEK_APPLY : IT -n> IT :=
+    λne e, Vis (E:=E) (subEff_opid op_peek_apply)
+             (subEff_ins (F:=delimE) (op:=op_peek_apply) (Next e))
+             (Empty_setO_rec _ ◎ (subEff_outs (F:=delimE) (op:=op_peek_apply))^-1).
+  Solve All Obligations with solve_proper.
+
+  Program Definition POP_CONTINUE_ : (IT -n> IT) -n> IT -n> IT :=
+    λne k e, Vis (E:=E) (subEff_opid op_pop_continue)
+             (subEff_ins (F:=delimE) (op:=op_pop_continue) (Next e))
+             (laterO_map k ◎ (subEff_outs (F:=delimE) (op:=op_pop_continue))^-1).
+  Solve All Obligations with solve_proper.
+
+  Program Definition POP_CONTINUE : IT -n> IT :=
+    POP_CONTINUE_ idfun.
+
+  Program Definition POP_DISCARD : IT -n> IT :=
+    λne e, Vis (E:=E) (subEff_opid op_pop_discard)
+             (subEff_ins (F:=delimE) (op:=op_pop_discard) (Next e))
+             (Empty_setO_rec _ ◎ (subEff_outs (F:=delimE) (op:=op_pop_discard))^-1).
+  Solve All Obligations with solve_proper.
+
+  Notation 𝒫 := (get_val POP_APPLY).
+  Notation ℛ := (get_val PEEK_APPLY).
+  Notation 𝒞 := (get_val POP_CONTINUE).
+  Notation ℱ := (get_val POP_DISCARD).
 
   (** ** RESET *)
 
@@ -140,7 +251,7 @@ Section constructors.
                                 laterO IT -n>
                                 IT :=
     λne k e, Vis (E:=E) (subEff_opid op_reset)
-               (subEff_ins (F := delimE) (op := op_reset) (laterO_map 𝒫 e))
+               (subEff_ins (F := delimE) (op := op_reset) e)
                (k ◎ subEff_outs (F := delimE) (op := op_reset)^-1).
   Solve Obligations with solve_proper.
 
@@ -153,7 +264,7 @@ Section constructors.
                                 (laterO IT -n> laterO IT) -n>
                                 IT :=
     λne f k, Vis (E:=E) (subEff_opid op_shift)
-             (subEff_ins (F:=delimE) (op:=op_shift) ((laterO_map $ 𝒫) ◎ f))
+             (subEff_ins (F:=delimE) (op:=op_shift) f)
              (k ◎ (subEff_outs (F:=delimE) (op:=op_shift))^-1).
   Solve All Obligations with solve_proper.
 
@@ -186,7 +297,10 @@ Section constructors.
 
 End constructors.
 
-Notation 𝒫 := (get_val POP).
+Notation 𝒫 := (get_val POP_APPLY).
+Notation ℛ := (get_val PEEK_APPLY).
+Notation 𝒞 := (get_val POP_CONTINUE).
+Notation ℱ := (get_val POP_DISCARD).
 
 Section weakestpre.
   Context {sz : nat}.
@@ -208,7 +322,7 @@ Section weakestpre.
 
   Lemma wp_shift (σ : state) (f : (laterO IT -n> laterO IT) -n> laterO IT)
     (k : IT -n> IT) β {Hk : IT_hom k} Φ s :
-    laterO_map 𝒫 (f (laterO_map k)) ≡ Next β →
+    (f (laterO_map k)) ≡ Next β →
     has_substate σ -∗
     ▷ (£ 1 -∗ has_substate σ -∗ WP@{rs} β @ s {{ Φ }}) -∗
     WP@{rs} (k (SHIFT f)) @ s {{ Φ }}.
@@ -216,10 +330,15 @@ Section weakestpre.
     iIntros (Hp) "Hs Ha".
     unfold SHIFT. simpl.
     rewrite hom_vis.
-    iApply (wp_subreify_ctx_dep _ _ _ _ _ _ _ (laterO_map 𝒫 $ f (laterO_map k)) with "Hs").
+    iApply (wp_subreify_ctx_dep _ _ _ _ _ _ _ (f (laterO_map k)) with "Hs").
     {
-      simpl. do 2 f_equiv; last done. do 2 f_equiv.
-      rewrite ccompose_id_l. intro. simpl. by rewrite ofe_iso_21.
+      simpl. do 2 f_equiv; last done.
+      rewrite ccompose_id_l.
+      f_equiv.
+      intros ?.
+      simpl.
+      rewrite ofe_iso_21.
+      reflexivity.
     }
     { exact Hp. }
     iModIntro.
@@ -230,12 +349,12 @@ Section weakestpre.
     Φ s :
     has_substate σ -∗
     ▷ (£ 1 -∗ has_substate ((laterO_map k) :: σ) -∗
-       WP@{rs} 𝒫 e @ s {{ Φ }}) -∗
+       WP@{rs} e @ s {{ Φ }}) -∗
     WP@{rs} k $ (RESET (Next e)) @ s {{ Φ }}.
   Proof.
     iIntros "Hs Ha".
     unfold RESET. simpl. rewrite hom_vis.
-    iApply (wp_subreify_ctx_dep _ _ _ _ _ _ _ (Next $ 𝒫 e) with "Hs").
+    iApply (wp_subreify_ctx_dep _ _ _ _ _ _ _ (Next $ e) with "Hs").
     - simpl. repeat f_equiv. rewrite ccompose_id_l.
       trans ((laterO_map k) :: σ); last reflexivity.
       f_equiv. intro. simpl. by rewrite ofe_iso_21.
@@ -243,34 +362,166 @@ Section weakestpre.
     - iApply "Ha".
   Qed.
 
-  Lemma wp_pop_end (v : IT)
-    {HV : AsVal v}
+  Lemma wp_pop_apply_end (e : IT)
     Φ s :
-    has_substate [] -∗
-    ▷ (£ 1 -∗ has_substate [] -∗ WP@{rs} v @ s {{ Φ }}) -∗
-    WP@{rs} 𝒫 v @ s {{ Φ }}.
+    has_substate []
+    -∗ ▷ (£ 1 -∗ has_substate [] -∗ WP@{rs} e @ s {{ Φ }})
+    -∗ WP@{rs} POP_APPLY e @ s {{ Φ }}.
   Proof.
     iIntros "Hs Ha".
-    rewrite get_val_ITV. simpl.
-    iApply (wp_subreify_ctx_dep _ _ _ _ _ _ _ ((Next v)) with "Hs").
+    iApply (wp_subreify_ctx_dep _ _ _ _ _ _ _ ((Next e)) with "Hs").
     - simpl. reflexivity.
     - reflexivity.
     - done.
   Qed.
 
-  Lemma wp_pop_cons (σ : state) (v : IT) (k : IT -n> IT)
-    {HV : AsVal v}
+  Lemma wp_pop_apply_cons (σ : state) (e : IT) (k : IT -n> IT)
     Φ s :
-    has_substate ((laterO_map k) :: σ) -∗
-    ▷ (£ 1 -∗ has_substate σ -∗ WP@{rs} k $ v @ s {{ Φ }}) -∗
-    WP@{rs} 𝒫 v @ s {{ Φ }}.
+    has_substate ((laterO_map k) :: σ)
+    -∗ ▷ (£ 1 -∗ has_substate σ -∗ WP@{rs} k $ e @ s {{ Φ }})
+    -∗ WP@{rs} POP_APPLY e @ s {{ Φ }}.
   Proof.
     iIntros "Hs Ha".
-    rewrite get_val_ITV. simpl.
-    iApply (wp_subreify_ctx_dep _ _ _ _ _ _ _ ((laterO_map k (Next v))) with "Hs").
+    iApply (wp_subreify_ctx_dep _ _ _ _ _ _ _ ((laterO_map k (Next e))) with "Hs").
     - simpl. reflexivity.
     - reflexivity.
     - done.
+  Qed.
+
+  Lemma wp_peek_apply_end (e : IT)
+    Φ s :
+    has_substate []
+    -∗ ▷ (£ 1 -∗ has_substate [] -∗ WP@{rs} e @ s {{ Φ }})
+    -∗ WP@{rs} PEEK_APPLY e @ s {{ Φ }}.
+  Proof.
+    iIntros "Hs Ha".
+    iApply (wp_subreify_ctx_dep _ _ _ _ _ _ _ ((Next e)) with "Hs").
+    - simpl. reflexivity.
+    - reflexivity.
+    - done.
+  Qed.
+
+  Lemma wp_peek_apply_cons (σ : state) (e : IT) (k : IT -n> IT)
+    Φ s :
+    has_substate ((laterO_map k) :: σ)
+    -∗ ▷ (£ 1 -∗ has_substate ((laterO_map k) :: σ) -∗ WP@{rs} k $ e @ s {{ Φ }})
+    -∗ WP@{rs} PEEK_APPLY e @ s {{ Φ }}.
+  Proof.
+    iIntros "Hs Ha".
+    iApply (wp_subreify_ctx_dep _ _ _ _ _ _ _ ((laterO_map k (Next e))) with "Hs").
+    - simpl. reflexivity.
+    - reflexivity.
+    - done.
+  Qed.
+
+  Lemma wp_pop_continue (e : IT) σ
+    Φ s :
+    has_substate σ
+    -∗ ▷ (£ 1 -∗ has_substate (tail σ) -∗ WP@{rs} e @ s {{ Φ }})
+    -∗ WP@{rs} POP_CONTINUE e @ s {{ Φ }}.
+  Proof.
+    iIntros "Hs Ha".
+    destruct σ.
+    - iApply (wp_subreify_ctx_dep _ _ _ _ _ _ _ ((Next e)) with "Hs").
+      + simpl; rewrite ofe_iso_21 later_map_Next; reflexivity.
+      + reflexivity.
+      + done.
+    - iApply (wp_subreify_ctx_dep _ _ _ _ _ _ _ ((Next e)) with "Hs").
+      + simpl; rewrite ofe_iso_21 later_map_Next; reflexivity.
+      + reflexivity.
+      + done.
+  Qed.
+
+  Lemma wp_pop_discard (e : IT) σ
+    Φ s :
+    has_substate σ
+    -∗ ▷ (£ 1 -∗ has_substate (tail σ) -∗ WP@{rs} e @ s {{ Φ }})
+    -∗ WP@{rs} POP_DISCARD e @ s {{ Φ }}.
+  Proof.
+    iIntros "Hs Ha".
+    destruct σ.
+    - iApply (wp_subreify_ctx_dep _ _ _ _ _ _ _ ((Next e)) with "Hs").
+      + simpl.
+        reflexivity.
+      + reflexivity.
+      + done.
+    - iApply (wp_subreify_ctx_dep _ _ _ _ _ _ _ ((Next e)) with "Hs").
+      + simpl.
+        reflexivity.
+      + reflexivity.
+      + done.
+  Qed.
+
+  Lemma wp_pop_apply_end' (v : IT)
+    {HV : AsVal v}
+    Φ s :
+    has_substate []
+    -∗ ▷ (£ 1 -∗ has_substate [] -∗ WP@{rs} v @ s {{ Φ }})
+    -∗ WP@{rs} 𝒫 v @ s {{ Φ }}.
+  Proof.
+    iIntros "Hs Ha".
+    rewrite get_val_ITV. simpl.
+    iApply (wp_pop_apply_end with "Hs Ha").
+  Qed.
+
+  Lemma wp_pop_apply_cons' (σ : state) (v : IT) (k : IT -n> IT)
+    {HV : AsVal v}
+    Φ s :
+    has_substate ((laterO_map k) :: σ)
+    -∗ ▷ (£ 1 -∗ has_substate σ -∗ WP@{rs} k $ v @ s {{ Φ }})
+    -∗ WP@{rs} 𝒫 v @ s {{ Φ }}.
+  Proof.
+    iIntros "Hs Ha".
+    rewrite get_val_ITV. simpl.
+    iApply (wp_pop_apply_cons with "Hs Ha").
+  Qed.
+
+  Lemma wp_peek_apply_end' (v : IT)
+    {HV : AsVal v}
+    Φ s :
+    has_substate []
+    -∗ ▷ (£ 1 -∗ has_substate [] -∗ WP@{rs} v @ s {{ Φ }})
+    -∗ WP@{rs} ℛ v @ s {{ Φ }}.
+  Proof.
+    iIntros "Hs Ha".
+    rewrite get_val_ITV. simpl.
+    iApply (wp_peek_apply_end with "Hs Ha").
+  Qed.
+
+  Lemma wp_peek_apply_cons' (σ : state) (v : IT) (k : IT -n> IT)
+    {HV : AsVal v}
+    Φ s :
+    has_substate ((laterO_map k) :: σ)
+    -∗ ▷ (£ 1 -∗ has_substate ((laterO_map k) :: σ) -∗ WP@{rs} k $ v @ s {{ Φ }})
+    -∗ WP@{rs} ℛ v @ s {{ Φ }}.
+  Proof.
+    iIntros "Hs Ha".
+    rewrite get_val_ITV. simpl.
+    iApply (wp_peek_apply_cons with "Hs Ha").
+  Qed.
+
+  Lemma wp_pop_continue' (v : IT) σ
+    {HV : AsVal v}
+    Φ s :
+    has_substate σ
+    -∗ ▷ (£ 1 -∗ has_substate (tail σ) -∗ WP@{rs} v @ s {{ Φ }})
+    -∗ WP@{rs} 𝒞 v @ s {{ Φ }}.
+  Proof.
+    iIntros "Hs Ha".
+    rewrite get_val_ITV. simpl.
+    iApply (wp_pop_continue with "Hs Ha").
+  Qed.
+
+  Lemma wp_pop_discard' (v : IT) σ
+    {HV : AsVal v}
+    Φ s :
+    has_substate σ
+    -∗ ▷ (£ 1 -∗ has_substate (tail σ) -∗ WP@{rs} v @ s {{ Φ }})
+    -∗ WP@{rs} ℱ v @ s {{ Φ }}.
+  Proof.
+    iIntros "Hs Ha".
+    rewrite get_val_ITV. simpl.
+    iApply (wp_pop_discard with "Hs Ha").
   Qed.
 
   Lemma wp_app_cont (σ : state) (e : laterO IT) (k' : laterO (IT -n> IT))
